qr

QR/Basics.ec
@@ -6,6 +6,7 @@ require  GenericSigmaProtocol.
 
 require import ZModP.
 clone include ZModRing.         (* must use ring since in ZModField QR is efficiently computable *)
+(* import DZmodP. *)
 
 abbrev invertible = unit.           (* more intuitive synonym *)
 
@@ -15,25 +16,19 @@ type qr_com  = zmod.
 type qr_resp = zmod.
 
 
-op IsSqRoot (Ny : qr_prob) (w : qr_wit) = Ny  = (w * w).
-op IsQR (Ny : qr_prob) = exists w, IsSqRoot Ny w /\ invertible Ny.
-
-
 op ZNS_dist :  (zmod * zmod) distr.
 
-axiom d_prop0  : is_uniform (ZNS_dist).
+axiom d_prop0  : is_uniform ZNS_dist.
 axiom d_prop1 r rr :  (r, rr) \in ZNS_dist => r * r = rr.
 axiom d_prop3 (r rr : zmod) :  r * r = rr => (r, rr) \in ZNS_dist.
 axiom d_prop4  r rr :  (r, rr) \in ZNS_dist => unit rr.
 axiom d_prop5 : weight (ZNS_dist) = 1%r.
 
 
-axiom qr_prop1 (x : zmod) : unit  x => x * (inv x)  = one.
-axiom qr_prop2 (x y w : zmod) : unit y => IsSqRoot (y) w => unit w.
-axiom qr_prop3 (w : zmod) : unit  w => inv  (w * w) = (inv w) * (inv w).
-axiom qr_prop5 (x y r : zmod) : IsQR x => unit x => !IsQR y => unit y => x * y  <> r * r.
 
-axiom qr_prop11 (x : zmod) : unit x => (inv x) * x = one.
+op completeness_relation = fun Ny w => Ny = (w * w) /\ invertible Ny.
+op soundness_relation    = fun Ny w => Ny = (w * w) /\ invertible Ny.
+op zk_relation           = fun Ny w => Ny = (w * w) /\ invertible Ny.
 
 
 (* Honest Vrifier  *)
@@ -42,9 +37,6 @@ op qr_verify (p : qr_prob) (c : qr_com) (b : bool) (r : qr_resp) : bool =
   else unit c /\ c = r * r.
 
 op verify_transcript = fun p (x : qr_com * bool * qr_resp) => qr_verify p x.`1 x.`2 x.`3.
-op soundness_relation    = fun Ny w => IsSqRoot Ny w /\ invertible Ny.
-op completeness_relation = fun Ny w => IsSqRoot Ny w /\ invertible Ny.
-op zk_relation           = fun Ny w => IsSqRoot Ny w /\ invertible Ny.
 
 clone export GenericSigmaProtocol as FiatShamir with 
   type statement       <- qr_prob,
@@ -57,6 +49,33 @@ clone export GenericSigmaProtocol as FiatShamir with
   op soundness_relation    <- soundness_relation,
   op completeness_relation <- completeness_relation,
   op zk_relation           <- zk_relation.
+
+
+
+lemma qr_prop1 (x : zmod) : unit x => x * (inv x)  = one. smt. qed.
+lemma qr_prop2 (x y w : zmod) : unit y => y = w * w => unit w. smt. qed.
+lemma qr_prop3 (w : zmod) : unit  w => inv (w * w) = (inv w) * (inv w). smt. qed.
+lemma qr_prop11 (x : zmod) : unit x => (inv x) * x = one. smt. qed.
+lemma qr_prop5 (x y r : zmod) : in_language completeness_relation x 
+  => !in_language completeness_relation y => unit y => x * y  <> r * r.
+progress.
+elim H. progress. 
+case (x * y = r * r). elim H.
+move => H xinv.
+pose w := witness.
+rewrite  H. 
+have iw : invertible witness.  smt.
+move => eq.
+have eq2 :  (inv w) * w * w * y = (inv w) * r * r. smt.
+have eq3 :  w * y = (inv w) * r * r. smt.
+clear eq2 eq.
+have eq4 :  (inv w) * w * y = ((inv w) * r) * (inv w) * r. smt.
+have eq5 :  y = ((inv w) * r) * ((inv w) * r). smt.
+apply H0. exists (inv w * r). split.
+apply eq5. auto.
+auto.
+qed.
+
 
 
 (* Honest Prover  *)
