QR/PoK.ec
@@ -13,7 +13,7 @@ declare module P <: RewMaliciousProver {-HV}.
 declare axiom P_response_ll : islossless P.response.
 
 lemma qr_computational_PoK &m  s: 
-  Pr[Extractor(P).extract(s) @ &m : IsSqRoot s res /\ unit s] >=
+  Pr[Extractor(P).extract(s) @ &m : soundness_relation s res ] >=
    (Pr[Soundness(P, HV).run(s) @ &m : res]^2
      - (1%r/2%r) * Pr[Soundness(P, HV).run(s) @ &m : res]).
 apply (SST.Perfect.PoK_from_special_soundness P  _ _ &m s  ).  apply P_response_ll. 
